program_logic/viewshifts.v
@@ -1,11 +1,11 @@
 From iris.program_logic Require Export invariants.
 From iris.proofmode Require Import tactics.
 
-Definition vs `{irisG Λ Σ} (E1 E2 : coPset) (P Q : iProp Σ) : iProp Σ :=
+Definition vs `{invG Σ} (E1 E2 : coPset) (P Q : iProp Σ) : iProp Σ :=
   (□ (P -★ |={E1,E2}=> Q))%I.
-Arguments vs {_ _ _} _ _ _%I _%I.
+Arguments vs {_ _} _ _ _%I _%I.
 
-Instance: Params (@vs) 5.
+Instance: Params (@vs) 4.
 Notation "P ={ E1 , E2 }=> Q" := (vs E1 E2 P Q)
   (at level 99, E1,E2 at level 50, Q at level 200,
    format "P  ={ E1 , E2 }=>  Q") : uPred_scope.
@@ -21,7 +21,7 @@ Notation "P ={ E }=> Q" := (True ⊢ P ={E}=> Q)%I
    format "P  ={ E }=>  Q") : C_scope.
 
 Section vs.
-Context `{irisG Λ Σ}.
+Context `{invG Σ}.
 Implicit Types P Q R : iProp Σ.
 Implicit Types N : namespace.
 
