program_logic/weakestpre.v
@@ -1,9 +1,25 @@
-From iris.program_logic Require Export fancy_updates.
-From iris.program_logic Require Import wsat.
+From iris.program_logic Require Export fancy_updates language.
 From iris.base_logic Require Import big_op.
-From iris.prelude Require Export coPset.
 From iris.proofmode Require Import tactics classes.
+From iris.algebra Require Import auth.
 Import uPred.
+
+Class irisG' (Λstate : Type) (Σ : gFunctors) : Set := IrisG {
+  iris_invG :> invG Σ;
+  state_inG :> inG Σ (authR (optionUR (exclR (leibnizC Λstate))));
+  state_name : gname;
+}.
+Notation irisG Λ Σ := (irisG' (state Λ) Σ).
+
+Definition ownP `{irisG' Λstate Σ} (σ : Λstate) : iProp Σ :=
+  own state_name (◯ (Excl' σ)).
+Typeclasses Opaque ownP.
+Instance: Params (@ownP) 3.
+
+Definition ownP_auth `{irisG' Λstate Σ} (σ : Λstate) : iProp Σ :=
+  own state_name (● (Excl' (σ:leibnizC Λstate))).
+Typeclasses Opaque ownP_auth.
+Instance: Params (@ownP_auth) 4.
 
 Definition wp_pre `{irisG Λ Σ}
     (wp : coPset -c> expr Λ -c> (val Λ -c> iProp Σ) -c> iProp Σ) :
@@ -96,6 +112,24 @@ Implicit Types Φ : val Λ → iProp Σ.
 Implicit Types v : val Λ.
 Implicit Types e : expr Λ.
 
+(* Physical state *)
+Lemma ownP_twice σ1 σ2 : ownP σ1 ★ ownP σ2 ⊢ False.
+Proof. rewrite /ownP own_valid_2. by iIntros (?). Qed.
+Global Instance ownP_timeless σ : TimelessP (@ownP (state Λ) Σ _ σ).
+Proof. rewrite /ownP; apply _. Qed.
+
+Lemma ownP_agree σ1 σ2 : ownP_auth σ1 ★ ownP σ2 ⊢ σ1 = σ2.
+Proof.
+  rewrite /ownP /ownP_auth own_valid_2 -auth_both_op.
+  by iIntros ([[[] [=]%leibniz_equiv] _]%auth_valid_discrete).
+Qed.
+Lemma ownP_update σ1 σ2 : ownP_auth σ1 ★ ownP σ1 ==★ ownP_auth σ2 ★ ownP σ2.
+Proof.
+  rewrite /ownP -!own_op.
+  by apply own_update, auth_update, option_local_update, exclusive_local_update.
+Qed.
+
+(* Weakest pre *)
 Lemma wp_unfold E e Φ : WP e @ E {{ Φ }} ⊣⊢ wp_pre wp E e Φ.
 Proof. rewrite wp_eq. apply (fixpoint_unfold wp_pre). Qed.
 
